LowStar.Queue: find
+ Tactics
+ LowStar.Loops: rec_while

Learn.LowStar.Loops.fst
@@ -9,9 +9,9 @@ open FStar.HyperStack.ST
 
 
 (* [reverse_for] *)
-(* implémentation de [C.Loops.reverse_for] avec [C.Loops.for] pour permettre l'extraction *)
+(* implementation of [C.Loops.reverse_for] using [C.Loops.for] for the extraction *)
 
-inline_for_extraction
+noextract inline_for_extraction
 let reverse_for (start:U32.t) (finish:U32.t{U32.v finish <= U32.v start})
     (inv:HS.mem -> nat -> Type0)
     (f:(i:U32.t{U32.(v start >= v i /\ v i > v finish)}) -> Stack unit
@@ -25,16 +25,16 @@ let reverse_for (start:U32.t) (finish:U32.t{U32.v finish <= U32.v start})
                 (fun i -> f U32.(start -^ i))
   
 
-(* [rec_reverse_for] *)
+(* [tail_rec_post h1 post1 post0] expresses the fact that a tail-recursive call (in the exit state [h1] of the
+   current step) establish (with its post-condition [post1]) the post-condition [post0] of the current step. *)
 
-(* TODO? relation St entre h1 et h2 *)
 let tail_rec_post (#a : Type) (h1 : HS.mem)
-  (post1 : a -> HS.mem -> Tot prop) (post0 : a -> HS.mem -> Tot prop)
+  (post1 : a -> HS.mem -> GTot prop) (post0 : a -> HS.mem -> GTot prop)
   : Tot prop
   = U.hide_prop (forall x h2. post1 x h2 /\ equal_stack_domains h1 h2 ==> post0 x h2)
 
 let tail_rec_postI (#a : Type) (h1 : HS.mem)
-  (post1 : a -> HS.mem -> Tot prop) (post0 : a -> HS.mem -> Tot prop)
+  (post1 : a -> HS.mem -> GTot prop) (post0 : a -> HS.mem -> GTot prop)
   (pf : (x:a) -> (h2:HS.mem) -> Lemma (requires post1 x h2 /\ equal_stack_domains h1 h2) (ensures post0 x h2))
   : Lemma (ensures tail_rec_post #a h1 post1 post0)
   = U.hide_propI_by (forall x h2. post1 x h2 /\ equal_stack_domains h1 h2 ==> post0 x h2) (fun () ->
@@ -43,13 +43,20 @@ let tail_rec_postI (#a : Type) (h1 : HS.mem)
             with pf0. pf x h2
     )
 
-(* [i] est le premier argument de pre/post pour faciliter le passage à [tail_rec_post] *)
+let tail_rec_postD #a h1 post1 post0 x h2
+  : Lemma (requires tail_rec_post #a h1 post1 post0)
+          (ensures post1 x h2 /\ equal_stack_domains h1 h2 ==> post0 x h2)
+  = U.hide_propD (forall x h2. post1 x h2 /\ equal_stack_domains h1 h2 ==> post0 x h2)
 
-inline_for_extraction
-let rec_reverse_for (start : U32.t) (finish : U32.t{U32.(v finish <= v start)}) (#a : Type)
-    (pre  : (i:nat{U32.(v start >= i /\ i >= v finish)}) -> HS.mem -> prop)
+(* [rec_reverse_for] *)
+
+(* [i] is the first parameter of [pre]&[post] to be directly used with [tail_rec_post] *)
+
+noextract inline_for_extraction
+let rec_reverse_for_st (start : U32.t) (finish : U32.t{U32.(v finish <= v start)}) (#a : Type)
+    (pre  : (i:nat{U32.(v start >= i /\ i >= v finish)}) -> HS.mem -> GTot prop)
     (post : (i:nat{U32.(v start >= i /\ i >= v finish)}) -> (h0:HS.mem) -> a -> HS.mem ->
-            Pure prop (requires pre i h0) (ensures fun _ -> True))
+            Ghost prop (requires pre i h0) (ensures fun _ -> True))
     (body : (i:U32.t{U32.(v start >= v i /\ v i > v finish)}) -> Stack unit
               (requires fun h0       -> pre (U32.v i) h0)
               (ensures  fun h0 () h1 -> pre (U32.v i - 1) h1 /\
@@ -95,3 +102,94 @@ let rec_reverse_for (start : U32.t) (finish : U32.t{U32.(v finish <= v start)}) 
     U.assert_by (post (U32.v start) h0 rt h2)
               (fun () -> U.hide_propD (inv_p h1 (U32.v finish)));
     rt
+
+
+(* [rec_while] *)
+
+(* We require that [test] does not modify the state ([h0' == h0]) because [body]&[exit] need to refer to [h0].
+   We could allow [h0' =!= h0] if we had a way to store [h0] (without modifying the state) in order to give it
+   to [body]&[exit]. Anyway, the extraction seems to remove any expression with side-effects from the guard (by
+   duplicating it). *)
+noextract inline_for_extraction
+let rec_while_st (#a : Type)
+    (pre       : HS.mem -> GTot prop)
+    (post_test : (h0:HS.mem) -> bool ->
+                   Ghost prop (requires pre h0) (ensures fun _ -> True))
+    (post      : (h0:HS.mem) -> a -> HS.mem ->
+                   Ghost prop (requires pre h0) (ensures fun _ -> True))
+    (test : unit -> Stack bool
+              (requires fun h0       -> pre h0)
+              (ensures  fun h0 b h0' -> h0' == h0 /\
+                                     post_test h0 b))
+    (body : unit -> Stack unit
+              (requires fun h0       -> pre h0 /\ post_test h0 true)
+              (ensures  fun h0 () h1 -> pre h1 /\
+                                     tail_rec_post h1 (post h1) (post h0)))
+    (exit : unit -> ST a
+              (requires fun h0       -> pre h0 /\ post_test h0 false)
+              (ensures  fun h0 x h1  -> post h0 x h1))
+  : ST a (requires fun h0      -> pre  h0)
+         (ensures  fun h0 x h1 -> post h0 x h1)
+  =
+    let h0 = ST.get () in
+    let test_pre h1 =
+      pre h1 /\
+      (forall x h2 . post h1 x h2 /\ equal_stack_domains h1 h2 ==> post h0 x h2)
+    in let test_post b h1 =
+      test_pre h1 /\
+      post_test h1 b
+    in
+    let test' () : Stack bool
+              (requires fun h1      -> test_pre h1)
+              (ensures  fun _ b h1' -> test_post b h1')
+      = test ()
+    in
+    let body' () : Stack unit
+              (requires fun h1      -> test_post true h1)
+              (ensures  fun _ () h2 -> test_pre h2)
+      =   let h1 = ST.get () in
+        body ();
+          let h2 = ST.get () in
+          introduce forall x h3 . post h2 x h3 /\ equal_stack_domains h2 h3 ==> post h0 x h3
+            with begin
+                 eliminate forall x h3 . post h1 x h3 /\ equal_stack_domains h1 h3 ==> post h0 x h3
+                      with x h3;
+                 tail_rec_postD h2 (post h2) (post h1) x h3
+            end
+    in
+    C.Loops.while #test_pre #test_post test' body';
+    exit ()
+
+
+noextract inline_for_extraction
+let rec_while (#a : Type)
+    (pre       : HS.mem -> GTot prop)
+    (post_test : (h0:HS.mem) -> bool ->
+                   Ghost prop (requires pre h0) (ensures fun _ -> True))
+    (post      : (h0:HS.mem) -> a -> HS.mem ->
+                   Ghost prop (requires pre h0) (ensures fun _ -> True))
+    (test : unit -> Stack bool
+              (requires fun h0       -> pre h0)
+              (ensures  fun h0 b h0' -> h0' == h0 /\
+                                     post_test h0 b))
+    (body : unit -> Stack unit
+              (requires fun h0       -> pre h0 /\ post_test h0 true)
+              (ensures  fun h0 () h1 -> pre h1 /\
+                                     tail_rec_post h1 (post h1) (post h0)))
+    (exit : unit -> Stack a
+              (requires fun h0       -> pre h0 /\ post_test h0 false)
+              (ensures  fun h0 x h1  -> post h0 x h1))
+  : Stack a (requires fun h0      -> pre  h0)
+            (ensures  fun h0 x h1 -> post h0 x h1)
+  =
+    let post' h0 x h1 : Ghost prop (requires pre h0) (ensures fun _ -> True) =
+        post h0 x h1 /\ ST.equal_domains h0 h1 in
+    rec_while_st pre post_test post'
+                 test
+                 (fun () ->
+                   let h0 = ST.get () in
+                   body ();
+                   let h1 = ST.get () in
+                   tail_rec_postI h1 (post' h1) (post' h0) (fun x h2 ->
+                     tail_rec_postD h1 (post h1) (post h0) x h2))
+                 exit
