Learn.LowStar.Queue.Impl.fst
@@ -8,6 +8,7 @@ module G   = FStar.Ghost
 module HS  = FStar.HyperStack
 module ST  = FStar.HyperStack.ST
 module U32 = FStar.UInt32
+module LLoops = Learn.LowStar.Loops
 
 open LowStar.BufferOps
 open FStar.HyperStack.ST
@@ -24,10 +25,20 @@ let malloc (a : Type) (r : HS.rid)
        (requires fun _       -> ST.is_eternal_region r)
        (ensures  fun h0 q h1 -> M.(modifies loc_none h0 h1 /\
                                 fresh_loc (loc_buffer q) h0 h1 /\
-                                loc_includes (loc_region_only true r) (loc_buffer q)) /\
+                                loc_includes (loc_region_only true r) (loc_buffer q) /\
+                                freeable q) /\
                              live_queue h1 q [])
   =
     B.malloc #(queue_st a) r ({q_exit = B.null; q_entry = B.null}) 1ul
+
+(* [free] *)
+
+let free (#a : Type) (q : queue a)
+  : ST  unit
+       (requires fun h      -> live_queue h q [] /\ M.freeable q)
+       (ensures  fun h b h' -> M.(modifies (loc_addr_of_buffer q) h h'))
+  =
+    B.free q
 
 (* [is_empty] *)
 
@@ -58,7 +69,7 @@ let enqueue (#a : Type) (x : B.pointer (cell a)) (q : queue a) (l : G.erased (ce
         let ini = G.hide (unsnoc_seg sg)._1 in
         let tls = G.hide (unsnoc_seg sg)._2 in
         sg_unapp ini tls;
-        let tl,_ = sg_uncons tls in
+        let tl = (sg_uncons tls)._1 in
         assert (loc_seg tls.segment == B.loc_buffer tl);
         assert (loc_seg sg.segment  == M.(loc_union (loc_seg ini.segment) (B.loc_buffer tl)));
       (q.(0ul)).q_entry.(0ul) <- {(q.(0ul)).q_entry.(0ul) with next = x};
@@ -79,7 +90,7 @@ let enqueue (#a : Type) (x : B.pointer (cell a)) (q : queue a) (l : G.erased (ce
 
 (* [dequeue] *)
 
-let dequeue (#a : Type) (x : B.pointer (cell a)) (q : queue a) (l : G.erased (cell_list a))
+let dequeue (#a : Type) (q : queue a) (l : G.erased (cell_list a))
   : Stack (B.pointer (cell a))
           (requires fun h0       -> wf_queue q l /\ live_queue h0 q l /\
                                  Cons? l)
@@ -100,10 +111,171 @@ let dequeue (#a : Type) (x : B.pointer (cell a)) (q : queue a) (l : G.erased (ce
       disjoint_mod_next_seg h0 h1 md sg');
     rt
 
+(* [find] *)
 
+#push-options "--ifuel 1"
+let rec find_gtot (#a:Type) (f:a -> GTot bool) (l:list a) : GTot (option (x:a{f x})) (decreases l)
+  = match l with
+  | [] -> None
+  | hd :: tl -> if f hd then Some #(x:a{f x}) hd else find_gtot f tl
+#pop-options
+
+
+inline_for_extraction
+let rec list_find_rec (#a : Type)
+         (p : cell_ptr a) (sg : G.erased (list_nil a))
+         (h0 : HS.mem) (* needed to specify [f] *)
+         (spec_f : (x : B.pointer (cell a) -> GTot bool))
+         (f : (x : B.pointer (cell a)) ->
+              Stack bool
+                    (requires fun h      -> h == h0 /\ B.live h x /\ L.memP x sg.segment)
+                    (ensures  fun h b h' -> h' == h /\ b = spec_f x))
+   : Stack (B.pointer_or_null (cell a))
+          (requires fun h       -> h == h0 /\ live_seg h sg /\ p == sg_entry sg)
+          (ensures  fun h rt h' -> h' == h /\
+                                rt == (match find_gtot spec_f sg.segment with
+                                       | Some p -> p | None -> B.null))
+   =
+     if B.is_null (sgn_entry p sg) then B.null
+     else begin
+         let tl = (sg_uncons (G.reveal sg))._2 in
+       if f p then p
+       else list_find_rec (sg_next p (G.reveal sg)) (G.reveal tl) h0 spec_f f
+     end
+
+#push-options "--z3rlimit 20"
+inline_for_extraction
+let list_find_loop (#a : Type)
+         (p : cell_ptr a) (sg0 : G.erased (list_nil a))
+         (h0  : HS.mem)
+         (spec_f : (x : B.pointer (cell a) -> GTot bool))
+         (f : (x : B.pointer (cell a)) ->
+              Stack bool
+                    (requires fun h -> M.(modifies loc_none h0 h) /\ B.live h x /\ L.memP x sg0.segment)
+                    (ensures  fun h b h' -> M.(modifies loc_none h h') /\ b = spec_f x))
+   : Stack (B.pointer_or_null (cell a))
+          (requires fun h       -> h == h0 /\ live_seg h sg0 /\ p == sg_entry sg0)
+          (ensures  fun h rt h' -> M.(modifies loc_none h h') /\
+                                rt == (match find_gtot spec_f sg0.segment with
+                                       | Some p -> p | None -> B.null))
+   =
+     push_frame ();
+       let h0' = ST.get () in
+     let it = B.alloca #(cell_ptr a & G.erased (list_nil a)) (p, sg0) 1ul in
+     let rt = B.alloca #(cell_ptr a) B.null 1ul in
+       let lloc = G.hide (M.(loc_union (loc_buffer it) (loc_buffer rt))) in
+     let pre h1 : prop =
+         M.(let (p, sg) = deref h1 it in
+         modifies loc_none h0 h1 /\
+         live h1 it /\ live h1 rt /\
+         live_seg h1 (deref h1 it)._2 /\
+         loc_disjoint (loc_buffer it) (loc_seg sg.segment) /\
+         p == sg_entry sg /\
+         (forall x . {:pattern (L.memP x sg0.segment)} L.memP x sg.segment ==> L.memP x sg0.segment))
+     in let post_test h1 (b:bool) : prop =
+         (Cons? (B.deref h1 it)._2.segment <==> b)
+     in let post h1 (x : cell_ptr a) h2 : prop =
+         let _,sg = B.deref h1 it in
+         let dflt = B.deref h1 rt in
+         M.(modifies lloc h1 h2) /\
+         x == (match find_gtot spec_f sg.segment with
+                     | Some p -> p | None -> dflt)
+     in
+     let test () : Stack bool
+              (requires fun h1       -> pre h1)
+              (ensures  fun h1 b h1' -> h1' == h1 /\ post_test h1 b)
+       =   let sg = (it.(0ul))._2 in
+         not (B.is_null (sgn_entry (it.(0ul))._1 sg))
+     in
+     let body () : Stack unit
+              (requires fun h1       -> pre h1 /\ Cons? (B.deref h1 it)._2.segment)
+              (ensures  fun h1 () h2 -> pre h2 /\
+                                     LLoops.tail_rec_post h2 (post h2) (post h1))
+       =   let h1 = ST.get () in
+           let sg = (it.(0ul))._2 in
+           let tl = (sg_uncons (G.reveal sg))._2 in
+         if f (sgn_entry (it.(0ul))._1 sg)
+         then begin
+           rt.(0ul) <- (it.(0ul))._1;
+           it.(0ul) <- (B.null, G.hide (empty_list a))
+         end else begin
+           it.(0ul) <- (sg_next (it.(0ul))._1 (G.hide (G.reveal sg)), (G.hide (G.reveal tl)))
+         end;
+           let h2 = ST.get () in
+           assert M.(modifies lloc h0 h2);
+           U.assert_by M.(modifies loc_none h0 h2) (fun () ->
+               assert M.(fresh_loc (loc_union (loc_buffer it) (loc_buffer rt)) h0 h1));
+           LLoops.tail_rec_postI h2 (post h2) (post h1) (fun x h3 -> ())
+     in
+     let rt_v = LLoops.rec_while pre post_test post  test body (fun () -> rt.(0ul)) in
+     pop_frame ();
+     rt_v
+#pop-options
+
+
+inline_for_extraction
+let find (#a : Type)
+         (q : queue a) (l : G.erased (cell_list a))
+         (h0  : HS.mem)
+         (spec_f : (x : B.pointer (cell a) -> GTot bool))
+         (f : (x : B.pointer (cell a)) ->
+              Stack bool
+                    (requires fun h -> M.(modifies loc_none h0 h) /\ B.live h x /\ L.memP x l)
+                    (ensures  fun h b h' -> M.(modifies loc_none h h') /\ b = spec_f x))
+  : Stack (B.pointer_or_null (cell a))
+          (requires fun h       -> h == h0 /\ live_queue h q l)
+          (ensures  fun h rt h' -> M.(modifies loc_none h h') /\
+                                rt == (match find_gtot spec_f l with
+                                       | Some p -> p | None -> B.null))
+  = list_find_loop ((q.(0ul)).q_exit) (sg_of_cells l) h0 spec_f f
+ 
 (* ---------- *)
 
 let malloc_u32   = malloc    U32.t
 let is_empty_u32 = is_empty #U32.t
 let enqueue_u32  = enqueue  #U32.t
 let dequeue_u32  = dequeue  #U32.t
+
+let mem_42 (q : queue U32.t) (l : G.erased (cell_list U32.t))
+  : Stack (B.pointer_or_null (cell U32.t))
+          (requires fun h       -> live_queue h q l)
+          (ensures  fun h rt h' -> M.(modifies loc_none h h') /\
+                    rt == (match find_gtot (fun (c:B.pointer (cell U32.t)) -> (B.deref h c).data = 42ul) l with
+                           | Some p -> p | None -> B.null))
+  =   let h = ST.get () in
+    find q l h (fun c -> (B.deref h c).data = 42ul)
+               (fun c -> live_seg_cell h (sg_of_cells l) c; (c.(0ul)).data = 42ul)
+
+#push-options "--fuel 3 --z3rlimit 40"
+let test_queue_spec () : St unit
+  =
+    push_frame ();
+    let q = malloc U32.t HS.root in
+    let x0 = B.malloc #(cell U32.t) HS.root ({data = 5ul; next = B.null}) 1ul in
+    enqueue x0 q [];
+      (let h = ST.get () in assert (live_queue h q [x0]));
+      (let d = (x0.(0ul)).data in assert (d == 5ul));
+      (let f = mem_42 q [x0] in assert (f == B.null));
+      (let h0 = ST.get () in
+    x0.(0ul) <- {x0.(0ul) with data = 42ul};
+      (let h1 = ST.get () in
+       frame_seg_mod_data h0 h1 (sg_of_cells [x0]);
+       assert (live_queue h1 q [x0])));
+      (let f = mem_42 q [x0] in assert (f == x0));
+
+    let x12 = B.alloca #(cell U32.t) ({data = 7ul; next = B.null}) 2ul in
+    let x1 = B.sub x12 0ul 1ul in let x2 = B.sub x12 1ul 1ul in
+    enqueue x1 q [x0];
+      (let h0 = ST.get () in assert (live_queue h0 q [x0; x1]);
+    x2.(0ul) <- {x2.(0ul) with data = 8ul};
+      let h1 = ST.get () in
+      frame_seg h0 h1 (sg_of_cells [x0; x1]) (M.loc_buffer x2);
+      assert (live_queue h1 q [x0; x1]));
+    let x0' = dequeue q [x0; x1] in
+      assert (x0' == x0);
+    B.free x0;
+    let x1' = dequeue q [x1] in
+      (assert (x1' == x1); let d = (x1.(0ul)).data in assert (d = 7ul));
+    pop_frame ();
+    free q
+#pop-options
