Learn.Tactics.Test.fst
@@ -3,35 +3,112 @@ module Learn.Tactics.Test
 module T   = FStar.Tactics
 module Tuq = Learn.Tactics.Unsquash
 
+open FStar.Calc
 open FStar.List.Pure
-open Learn.List
 
 
 [@expect_failure]
 let () = assert ((True ==> False) ==> (forall (x : nat) . False))
-             by (let h = impI () in
-                 let x = allI () in revert ();
-                 let _ = impD h in
-                 qed ())
+           by Tuq.(let h = impI () in
+                   let x = allI () in T.revert ();
+                   let _ = impD h in
+                   T.qed ())
 
 [@expect_failure]
 let () = assert ((True /\ False) ==> (forall (x : nat) . False))
-             by (let h = impI () in
-                 let x = allI () in revert ();
-                 let _ = andD h in
-                 qed ())
+           by Tuq.(let h = impI () in
+                   let x = allI () in T.revert ();
+                   let _ = andD h in
+                   T.qed ())
 
-let test0 (a : Type) (f : a -> prop) (hd : a) (tl : list a) : unit =
+[@expect_failure]
+let () = assert ((forall (x y:nat) . False) ==> (forall (x : nat) . True))
+           by Tuq.(let _ = hyp_arrow_morph_right (fun x p -> allD p) (allD (impI ())) in
+                   T.qed ())
+
+[@expect_failure]
+let () = assert ((True ==> False) /\ (forall (x : int) . True))
+           by Tuq.(andI1 ();
+                   goal_pair_morph (fun () -> let _ = impI() in T.revert ())
+                                   (fun () -> let _ = allI() in T.revert ());
+                   T.qed ())
+
+[@expect_failure]
+let () = assert (((True ==> False) /\ (forall (x:int) . True)) ==> False)
+           by Tuq.(let h = andD1 (impI ()) in
+                   let _ = hyp_pair_morph impD allD h in
+                   T.qed ())
+
+
+let test0 (a : Type) (f : a -> prop) (hd : a) (tl : list a) =
   assert (f hd /\ (forall (i:nat{i < length tl}). f (index tl i))
             ==> (forall (i:nat{i < length (hd :: tl)}) . f (index (hd :: tl) i)))
-      by (Tuq.(usq (Imp (And Nop (All Nop)) (All Nop)));
+      by (Tuq.(usq true true (Imp (And Nop (All Nop)) (All Nop)));
           Tuq.lbd_exact (`(fun h_hd h_tl i -> if i = 0 then h_hd else h_tl (i-1))))
 
-let test1 (a : Type) (f : a -> prop) (hd : a) (tl : list a) : unit =
+let test1 (a : Type) (f : a -> prop) (hd : a) (tl : list a) =
   assert (f hd /\ (forall (i:nat{i < length tl}). f (index tl i))
            <==> (forall (i:nat{i < length (hd :: tl)}) . f (index (hd :: tl) i)))
-      by (Tuq.(lbd_prf (iff (And Nop (All Nop)) (All Nop)))
+      by (Tuq.(lbd_prfs (`(_ /\ (forall i._) <==> (forall i._))))
               [(`(fun h_hd h_tl i -> if i = 0 then h_hd else h_tl (i-1)));
                (`(fun hi -> hi 0));
                (`(fun hi i -> hi (i+1)))])
-  
+
+let test2 (a : Type) (p : a -> a -> prop) =
+  assert ((forall (x y : a) . p x y) ==> (forall (x y : a) . p y x))
+    by (Tuq.(lbd_prf (`((forall x y._) ==> (forall x y._))))
+            (`(fun h x y -> h y x)))
+
+let test3 (p : nat -> prop) =
+  assert ((forall (i:nat) . p i) ==> p 0 /\ p 1)
+    by (Tuq.(usq false true (Imp (All Nop) (And Nop Nop)));
+        Tuq.lbd_exact (`(fun h -> (h 0, h 1))))
+
+let test4 (p q : nat -> prop) =
+  assert ((forall (i:nat) . p i /\ (p (i+1) ==> q i)) ==> p 0 /\ q 0)
+    by (Tuq.(lbd_prf (`((forall i._ /\ (_==>_)) ==> _ /\ _)))
+            (`(fun h -> (h 0)._1, (h 0)._2 (h 1)._1)))
+
+let test5 (p q : prop) =
+  assert (p /\ (p ==> q) ==> p /\ q)
+    by (Tuq.(lbd_prf (`(_ /\ (_ ==> _) ==> _ /\ _)))
+            (`(fun hp hq -> (hp, hq hp))))
+
+[@expect_failure 228] (* [tl] not found *)
+let test6 (a : Type) (f : a -> prop) (hd : a) (tl : list a) =
+   assert ((forall (i:nat{i < length (hd :: tl)}) . f (index (hd :: tl) i))
+           ==> f hd /\ (forall (i:nat{i < length tl}). f (index tl i)))
+      by (Tuq.(lbd_prf (`((forall i._) ==> _ /\ (forall i._))))
+              (`(fun h -> (h 0, (fun (i: nat{i < length tl}) -> h (i + 1))))))
+
+let test7 (f : nat -> prop) (i : nat) =
+  assert ((forall (j:nat) . f j) ==> f i)
+    by (T.revert ();
+        let i  = T.intro () in
+        let h  = T.implies_intro () in
+        let h' = T.instantiate h i in
+        T.hyp h')
+
+let test8 (p q r : prop) =
+  assert (p ==> (p ==> q /\ r) ==> r)
+    by (Tuq.(lbd_prf (`(_ ==> (_ ==> _ /\ _) ==> _)))
+            (`(fun hp hqr  -> (hqr hp)._2)))
+
+[@expect_failure]
+let test9 (a : Type) (l : list a) : unit
+  = match l with
+    | [] -> ()
+    | hd :: tl ->
+        assert (l == hd :: tl); (* OK *)
+        assert (l == hd :: tl)
+          by T.(dump "test9.1"; smt (); qed ()); (* OK *)
+        calc (==) {
+            l;
+          == {assert (l == hd :: tl)} (* OK *)
+            hd :: tl;
+        };
+        calc (==) {
+            l;
+          == {_ by T.(dump "test9.2"; smt (); qed ())} (* KO *)
+            hd :: tl;
+        }
