Learn.Tactics.Unsquash.fst
@@ -5,32 +5,31 @@ module F = FStar.Reflection.Formula
 open FStar.Tactics
 
 private
-let __pose (a:Type) (b:Type) (x : a) (f : a -> b) : b = f x
+let __pose (goal:Type) (#t:Type) (x : t) (f : t -> goal) : goal = f x
 
-(* TODO? force the instantiation of [b] *)
 let pose' (t:term) : Tac binder =
-    apply (`__pose);
+    apply (`__pose (`#(cur_goal ())));
     exact t;
     intro ()
 
 
-(* [allI] : introduces [forall (x : t) . p x] into [x:t |- squash (p x)] *)
+(* [allI] : introduces [forall (x : t) . p x] with [x:t |- squash (p x)] *)
 
 let allI : unit -> Tac binder = forall_intro
 
 (* [allD] : destructs [forall (x : t) . p x] into [(x : t) -> squash (p x)] *)
 
 private
-let __forall_usq #t (#pred : t -> Type0) (h : (forall x. pred x)) : x:t -> squash (pred x) =
+let __allD #t (#pred : t -> Type0) (h : (forall x. pred x)) : x:t -> squash (pred x) =
   fun x -> ()
 
 private
-let __forall_usq_sq #t (#pred : t -> Type0) (h : squash (forall x. pred x)) : x:t -> squash (pred x) =
+let __allD_sq #t (#pred : t -> Type0) (h : squash (forall x. pred x)) : x:t -> squash (pred x) =
   fun x -> ()
 
 let allD_keep (fa : term) : Tac binder =
-  try pose' (`__forall_usq_sq (`#fa)) with | _ ->
-  try pose' (`__forall_usq (`#fa)) with | _ ->
+  try pose' (`__allD_sq (`#fa)) with | _ ->
+  try pose' (`__allD    (`#fa)) with | _ ->
   fail "allD: could not unsquash"
 
 let allD (fa : binder) : Tac binder =
@@ -38,28 +37,29 @@ let allD (fa : binder) : Tac binder =
   clear fa;
   faa
 
+
 (* [impI] : introduces [a ==> b] with [_ : squash a |- squash b] *)
 
-private let imp_intro_lem (#a #b:Type) (prf : squash a -> squash b) : Lemma (a ==> b)
+private let __impI (#a #b:Type) (prf : squash a -> squash b) : Lemma (a ==> b)
   = introduce a ==> b with pf_a . prf pf_a
 
 let impI () : Tac binder =
-  apply_lemma (`imp_intro_lem);
+  apply_lemma (`__impI);
   intro ()
 
 (* [impD] : destructs [a ==> b] into [squash a -> squash b] *)
 
 private
-let __imp_usq (#a #b : Type) (h : (a ==> b)) : squash a -> squash b =
+let __impD (#a #b : Type) (h : (a ==> b)) : squash a -> squash b =
   fun pa -> ()
 
 private
-let __imp_usq_sq (#a #b : Type) (h : squash (a ==> b)) : squash a -> squash b =
+let __impD_sq (#a #b : Type) (h : squash (a ==> b)) : squash a -> squash b =
   fun pa -> ()
 
 let impD_keep (ip : term) : Tac binder =
-  try pose' (`__imp_usq_sq (`#ip)) with | _ ->
-  try pose' (`__imp_usq (`#ip)) with | _ ->
+  try pose' (`__impD_sq (`#ip)) with | _ ->
+  try pose' (`__impD    (`#ip)) with | _ ->
   fail "impD: could not unsquash"
 
 let impD (ip : binder) : Tac binder =
@@ -67,9 +67,18 @@ let impD (ip : binder) : Tac binder =
   clear ip;
   rt
 
+
 (* [andI] : introduces [a /\ b] with [squash a] and [squash b] *)
 
 let andI : unit -> Tac unit = split
+
+(* [andI1] : introduces [a /\ b] with [(squash a) & (squash b)] *)
+
+private let __andI1 (#a #b:Type) (prf : (squash a) & (squash b)) : Lemma (a /\ b)
+  = ()
+
+let andI1 () : Tac unit =
+  apply_lemma (`__andI1)
 
 (* [andD] : destrucs [a /\ b] into [squash a, squash b]
    Also works if the goal is not a squash. *)
@@ -95,7 +104,91 @@ let andD (b : binder) : Tac (binder & binder) =
   clear b;
   rt
 
-(* proof as lambda term *)
+(* [andD1] : destrucs [a /\ b] into [(squash a) & (squash b)] *)
+
+private
+let __andD1 (#a #b : Type) (h : (a /\ b)) : (squash a) & (squash b) =
+  (), ()
+
+private
+let __andD1_sq (#a #b : Type) (h : squash (a /\ b)) : (squash a) & (squash b) =
+  (), ()
+
+let andD1_keep (cj : term) : Tac binder =
+  try pose' (`__andD1_sq (`#cj)) with | _ ->
+  try pose' (`__andD1    (`#cj)) with | _ ->
+  fail "andD1: could not unsquash"
+
+let andD1 (cj : binder) : Tac binder =
+  let rt = andD1_keep cj in
+  clear cj;
+  rt
+
+
+(* [->] is a morphism in its target *)
+
+private
+let __hyp_arrow_morph_right (goal : Type) (#t : Type) (#p : t -> Type) (#q : t -> Type) (h : (x:t) -> p x)
+                            (f : (x:t) -> p x -> q x) (ct : ((x:t) -> q x) -> goal) : goal
+  = ct (fun x -> f x (h x)) 
+
+let hyp_arrow_morph_right
+    (f : binder(*x:t*) -> binder(*p x*) -> Tac binder(*q x*))
+    (ar : binder(*x:t -> p x*))
+  : Tac binder(*x:t -> q x*) =
+  apply (`__hyp_arrow_morph_right (`#(cur_goal ())) (`#ar));
+  begin let x = intro ()  in
+        let p = intro ()  in
+        let q = f x p in
+        exact q
+  end;
+  clear ar;
+  let ar = intro () in
+  norm_binder_type [] ar;
+  ar
+
+
+(* [&] is a morphism *)
+
+private
+let __goal_pair_morph (#p0 #p1 #q0 #q1 : Type) (f0 : p0 -> q0) (f1 : p1 -> q1) (x : p0 & p1) : q0 & q1
+  = (f0 x._1, f1 x._2)
+
+let goal_pair_morph (f0 : unit -> Tac unit(*q0 <- p0*)) (f1 : unit -> Tac unit(*q1 <- p1*))
+  : Tac unit(*q0&q1 <- p0&p1*)
+  = apply (`__goal_pair_morph);
+    begin let p0 = intro () in
+          f0 ();
+          exact p0
+    end;
+    begin let p1 = intro () in
+          f1 ();
+          exact p1
+    end
+
+private
+let __hyp_pair_morph (goal : Type) (#p0 #p1 #q0 #q1 : Type) (h : p0 & p1)
+                     (f0 : p0 -> q0) (f1 : p1 -> q1) (ct : (q0 & q1) -> goal) : goal
+  = ct (f0 h._1, f1 h._2)
+
+let hyp_pair_morph
+    (f0 : binder(*p0*) -> Tac binder(*q0*)) (f1 : binder(*p1*) -> Tac binder(*q1*))
+    (pr : binder(*p0&p1*))
+  : Tac binder(*q0&q1*) =
+  apply (`__hyp_pair_morph (`#(cur_goal ())) (`#pr));
+  begin let p0 = intro ()  in
+        let q0 = f0 p0 in
+        exact q0
+  end;
+  begin let p1 = intro ()  in
+        let q1 = f1 p1 in
+        exact q1
+  end;
+  clear pr;
+  intro ()
+           
+
+(* proof by a lambda term *)
 
 let lbd_exact : term -> Tac unit =
   t_exact false true
@@ -120,49 +213,113 @@ let rec usq_t_of_term (f:term) : Tac usq_t =
   | _ -> Nop
 
 (* TODO: equivalent of Coq's `;` instead of CPS *) 
-let rec unsquash_goal (d : usq_t) (ct : unit -> Tac unit) : Tac unit
+(* [sg] : split goal
+   [sh] : split hypotheses *)
+let rec unsquash_goal (sg : bool) (sh : bool) (d : usq_t) (ct : unit -> Tac unit) : Tac unit
   = match d with
     | Nop   -> ct ()
     | All d ->
           let x = allI () in
-          unsquash_goal d (fun () ->
+          unsquash_goal sg sh d (fun () ->
             revert (); (* x *)
             ct ())
     | Imp dh dg ->
           let h = impI () in
-          unsquash_goal dg (fun () ->
-            unsquash_hyp dh h;
+          unsquash_goal sg sh dg (fun () ->
+            unsquash_hyp sh dh h;
             ct ())
     | And dl dr ->
-          andI ();
-          iseq [(fun () -> unsquash_goal dl ct); (fun () -> unsquash_goal dr ct)]
-(* revert the transformed hypothesis *)
-and unsquash_hyp (d : usq_t) (h : binder) : Tac unit
-  = match d with
+          if sg then begin
+            andI ();
+            iseq [(fun () -> unsquash_goal sg sh dl ct);
+                  (fun () -> unsquash_goal sg sh dr ct)]
+          end else begin
+            andI1 ();
+            goal_pair_morph (fun () -> unsquash_goal false sh dl (fun () -> ()))
+                            (fun () -> unsquash_goal false sh dr (fun () -> ()));
+            ct ()
+          end
+
+(* revert the transformed hypothesis (which may be split into several hypotheses) *)
+and unsquash_hyp (sh : bool) (d : usq_t) (h : binder) : Tac unit
+  = let rev1 () : Tac unit =
+       let h = unsquash_hyp1 d h in
+       revert () (* h *)
+    in
+    if not sh then rev1 ()
+    else match d with
+    | Nop | All _ | Imp _ _ -> rev1 ()
+    | And dl dr ->
+          let hl,hr = andD h in
+          unsquash_hyp sh dr hr;
+          unsquash_hyp sh dl hl
+          
+(* return the transformed hypothesis *)
+and unsquash_hyp1 (d : usq_t) (h : binder) : Tac binder
+   = match d with
     | Nop ->
-          revert () (* h *)
-    | All Nop ->
+          h
+    | All d ->
           let h = allD h in
-          revert () (* h *)
-    | All _ ->
-          fail "AllD _ : Not implemented"
-    | Imp Nop Nop ->
+          hyp_arrow_morph_right (fun x p -> unsquash_hyp1 d p) h
+    | Imp Nop dr ->
           let h = impD h in
-          revert () (* h *)
+          hyp_arrow_morph_right (fun _ p -> unsquash_hyp1 dr p) h
     | Imp _ _ ->
           fail "ImpD _ _ : Not implemented"
     | And dl dr ->
-          let hl,hr = andD h in
-          unsquash_hyp dr hr;
-          unsquash_hyp dl hl
+          let h = andD1 h in
+          hyp_pair_morph (unsquash_hyp1 dl) (unsquash_hyp1 dr) h
 
-let usq (d : usq_t) : Tac unit = unsquash_goal d (fun () -> ())
+
+let usq (split_goal split_hyps : bool) (d : usq_t) : Tac unit
+  = unsquash_goal split_goal split_hyps d (fun () -> ())
+
+(* Representation of [usq_t] with [term] *)
+
+(* from FSTAR_HOME/examples/tactics/Preprocess.fst *)
+let is_fv (fv:string) (t:term) : Tac bool =
+  match t with
+  | Tv_FVar fv' ->
+    String.concat "." (inspect_fv fv') = fv
+  | _ -> false
+
+let rec term_to_usq_t (t : term) : Tac usq_t =
+  match inspect_ln t with
+  | Tv_App _ _ ->
+    begin match collect_app t with
+    | h, [arg0, Q_Explicit] ->
+           if is_fv (`%Prims.l_Forall) h then
+             let t' = match inspect_ln arg0 with
+                      | Tv_Abs _ t' -> t' | _ -> fail "term_to_usq_t.0"
+             in
+             All (term_to_usq_t t')
+           else fail "term_to_usq_t.1"
+    | h, [arg0, Q_Explicit; arg1, Q_Explicit] ->
+           if is_fv (`%Prims.l_imp) h then
+             Imp (term_to_usq_t arg0) (term_to_usq_t arg1)
+           else if is_fv (`%Prims.l_and) h then
+             And (term_to_usq_t arg0) (term_to_usq_t arg1)
+           else if is_fv (`%Prims.l_iff) h then
+             iff (term_to_usq_t arg0) (term_to_usq_t arg1)
+           else fail ("term_to_usq_t.2: "^term_to_string (quote h))
+    | h,args ->  fail ("term_to_usq_t.3: "^term_to_string (quote h)^"   "^term_to_string (quote args))
+    end
+  | Tv_Unknown -> Nop
+  | _ -> fail "term_to_usq_t.4"
+
+
+(*let () = assert True by (let d = term_to_usq_t (`(_ <==> _)) in print (term_to_string (quote d)); smt ()) *)
+
+let lbd_prf (d : term) (pf : term) : Tac unit
+  = usq false true (term_to_usq_t d);
+    lbd_exact pf
 
 let rec iter_list (#a : Type) (f : a -> Tac unit) (l : list a) : Tac unit =
   match l with
   | [] -> ()
   | hd :: tl -> f hd; iter_list f tl
 
-let lbd_prf (d : usq_t) (pfs : list term) : Tac unit
-  = usq d;
+let lbd_prfs (d : term) (pfs : list term) : Tac unit
+  = usq true true (term_to_usq_t d);
     iter_list lbd_exact pfs
