Learn.Util.fsti
@@ -8,7 +8,7 @@ val hide_propI_by (p : prop) (prf : unit -> Lemma (ensures p)) : Lemma (ensures 
 
 val hide_propD (p : prop) : Lemma (requires hide_prop p) (ensures p)
 
-val prop_equal (#a : Type) (p : a -> prop) (x y : a)
+val prop_equal (#a : Type) (p : a -> Type) (x y : a)
   : Lemma (requires x == y /\ p x) (ensures p y)
 
-val assert_by (p : prop) (prf : unit -> Lemma (ensures p)) : Lemma (ensures p)
+val assert_by (p : Type) (prf : unit -> Lemma (ensures p)) : Lemma (ensures p)
